

1 Part A: Calculus

1.1 Calculus-Q1

CQ1.1 Use the chain rule to calculate the gradient of

$$h(\sigma) = \frac{1}{2} \|f(\sigma) - y\|^3$$

where $\sigma \in \mathbb{R}^m$ and f is some arbitrary function from \mathbb{R}^m to \mathbb{R}^n .

CQ1.2 Compute the expression in the case where:

$$f(\sigma) = \begin{bmatrix} \sigma_1 \cdot \sigma_2 \\ \sigma_1^2 + \sigma_2^2 \\ \sigma_1 \end{bmatrix}$$

$$\sigma = \begin{bmatrix} 1 \\ 2 \end{bmatrix}, \quad y = \begin{bmatrix} 1 \\ 1 \\ 1 \end{bmatrix}$$

$$h(\sigma) = \frac{1}{2} \|r(\sigma)\|^3$$

let:

$$r(\sigma) = f(\sigma) - y, \quad g(u) = \frac{1}{2} \|u\|^3$$

hence:

$$h(\sigma) = g(r(\sigma))$$

let us find gradients:

$$\|u\| = (u \cdot u^T)^{\frac{1}{2}}$$

↙

$$g(u) = \frac{1}{2} \|u\|^3 = \frac{1}{2} (u \cdot u^T)^{\frac{3}{2}}$$

$$\begin{aligned} g'(u) &= \frac{1}{2} \cdot \frac{3}{2} \cdot (u \cdot u^T)^{\frac{1}{2}} \cdot (u \cdot u^T)' = \frac{1}{2} \cdot \frac{3}{2} \cdot (u \cdot u^T)^{\frac{1}{2}} \cdot (u^2)' \\ &= \frac{1}{2} \cdot \frac{3}{2} \cdot \|u\| \cdot 2u = \frac{3}{2} \|u\| \cdot u = \end{aligned}$$

let $u = r(\sigma)$:

$$g'(u) = \frac{3}{2} \|r(\sigma)\| r(\sigma)$$

we evaluate $f'(\sigma)$ as the jacobian:

$$J_f(\sigma) = \begin{bmatrix} \frac{\partial f_1}{\partial \sigma_1} & \dots & \frac{\partial f_1}{\partial \sigma_m} \\ \vdots & \ddots & \vdots \\ \frac{\partial f_n}{\partial \sigma_1} & \dots & \frac{\partial f_n}{\partial \sigma_m} \end{bmatrix} \in \mathbb{R}^{n \times m}.$$

$$f'(\sigma) = \begin{pmatrix} 2 & 1 \\ 2 & 4 \\ 1 & 0 \end{pmatrix}$$

we want to find gradient $h(\sigma)$
evaluated at:

$$f(\sigma) = \begin{bmatrix} \sigma_1 \cdot \sigma_2 \\ \sigma_1^2 + \sigma_2^2 \\ \sigma_1 \end{bmatrix}$$

$$\sigma = \begin{bmatrix} 1 \\ 2 \end{bmatrix}, \quad y = \begin{bmatrix} 1 \\ 1 \\ 1 \end{bmatrix}$$

by the chain rule:

$$h'(\sigma) = g'(r(\sigma)) \cdot r'(\sigma)$$

↓

$$h'(\sigma) = g'(r(\sigma)) \cdot f'(\sigma)$$

$$= \frac{3}{2} \|r(\sigma)\| \cdot r(\sigma) \cdot f'(\sigma)$$

$$= \frac{3}{2} \|r(\sigma)\| \cdot J_f(\sigma)^T \cdot r(\sigma)$$

let us evaluate:

$$\sigma = \begin{bmatrix} 1 \\ 2 \end{bmatrix} \quad y = \begin{pmatrix} 1 \\ 1 \\ 1 \end{pmatrix}$$

$$f(\sigma) = \begin{pmatrix} 2 \\ 5 \\ 1 \end{pmatrix} \rightarrow f'(\sigma) = \begin{pmatrix} 2 & 1 \\ 2 & 4 \\ 1 & 0 \end{pmatrix}$$

↓
 $r(\sigma) = \begin{pmatrix} 1 \\ 4 \\ 0 \end{pmatrix}$

$$h'(\sigma) = \frac{3}{2} \cdot \left\| \begin{pmatrix} 1 \\ 4 \\ 0 \end{pmatrix} \right\| \cdot \begin{pmatrix} 2 & 2 & 1 \\ 1 & 4 & 0 \end{pmatrix} \cdot \begin{pmatrix} 1 \\ 4 \\ 0 \end{pmatrix}$$

$$= \frac{3}{2} \cdot \sqrt{17} \cdot \begin{pmatrix} 10 \\ 17 \end{pmatrix}$$

1.2 Calculus-Q2

The softmax function $S: \mathbb{R}^k \rightarrow [0, 1]^k$, is defined as follows:

$$S(x)_j = \frac{e^{x_j}}{\sum_{l=1}^k e^{x_l}}$$

This function takes an input vector $x \in \mathbb{R}^d$ and outputs a probability vector (non-negative entries that sum up to 1), corresponding to the weight of original entries of x .

CQ2: Calculate the Jacobian of the softmax function S .

$$S'(x) = \begin{bmatrix} \frac{\partial S_1}{\partial x_1} & \dots & \frac{\partial S_1}{\partial x_k} \\ \vdots & & \vdots \\ \frac{\partial S_k}{\partial x_1} & \dots & \frac{\partial S_k}{\partial x_k} \end{bmatrix}$$

$$\text{let } z = \sum_{i=1}^k e^{x_i}$$

$$\begin{aligned} \frac{\partial S_i}{\partial x_j} &= \frac{\frac{1}{z} \cdot \frac{\partial}{\partial x_j} e^{x_i}}{\frac{\partial}{\partial x_j} z} = \frac{\frac{1}{z} \cdot \frac{\partial}{\partial x_j} (e^{x_i}) \cdot z - e^{x_i} \cdot \frac{1}{z} \cdot \frac{\partial}{\partial x_j} (z)}{z^2} \\ &= \frac{\delta_{ij} e^{x_i} z - e^{x_i} e^{x_j}}{z^2} \\ &= \frac{e^{x_i}}{z} \left(\delta_{ij} - \frac{e^{x_j}}{z} \right) \end{aligned}$$

$$\text{therefore } J_{ij} = \begin{cases} S(x)_i \cdot (1 - S(x)_i) & i=j \\ -\frac{e^{x_i} \cdot e^{x_j}}{z^2} = -S(x)_i \cdot S(x)_j & i \neq j \end{cases}$$

$$J = \begin{bmatrix} S(x_1) \cdot (1 - S(x_1)) & -S(x_1) \cdot S(x_2) & \dots & -S(x_1) \cdot S(x_k) \\ \vdots & S(x_2) \cdot (1 - S(x_2)) & \ddots & \vdots \\ \vdots & \vdots & \ddots & S(x_k) \cdot (1 - S(x_k)) \\ -S(x_k) \cdot S(x_1) & \dots & \dots & \dots \end{bmatrix}$$

$$* \frac{f(x)}{g(x)} = \frac{f'(x)g(x) - f(x)g'(x)}{g(x)^2}$$

$$\cdot (\sum e^{x_i})' = \sum (e^{x_i})' = \sum e^{x_i}$$

$$* * \frac{\partial}{\partial x_j} e^{x_i} = \begin{cases} e^{x_i} & i=j \\ 0 & i \neq j \end{cases}$$

$$\delta_{ij} = \begin{cases} 1 & i=j \\ 0 & i \neq j \end{cases}$$

$$\frac{\partial}{\partial x_j} (z) = \frac{1}{z} \sum e^{x_i} = \begin{cases} e^{x_j} & i=j \\ 0 & i \neq j \end{cases}$$